split, join

ulib/experimental/Steel.HigherArray0.fst
@@ -12,23 +12,6 @@ open Steel.Effect
 
 /// NOTE: This module is slated to have primitive Karamel extraction.
 
-(*
-/// Gather permissions on reference [r]
-let derive_composable (#o:inames)
-           (#a:Type u#1)
-           (#p:P.pcm a)
-           (r:ref a p)
-           (v0:a)
-           (v1:a)
-  : SteelGhost unit o
-           (R.pts_to r v0 `star` R.pts_to r v1)
-           (fun _ -> R.pts_to r v0 `star` R.pts_to r v1)
-           (fun _ -> True)
-           (fun _ _ _ -> FStar.PCM.composable p v0 v1)
-= R.gather r v0 v1;
-  R.split r _ v0 v1
-*)
-
 [@@noextract_to "krml"]
 let carrier (elt: Type u#a) : Tot Type =
   PM.map nat (P.fractional elt)
@@ -88,13 +71,28 @@ type ptr (elt: Type) = {
   offset: (offset: nat { offset <= U32.v base_len });
 }
 
-inline_for_extraction // Karamel should extract this to ptr, erasing the length and prf fields
+[@@erasable]
+let base_t (elt: Type) : Tot Type = Ghost.erased (U32.t & ref _ (pcm elt))
+let base_len (#elt: Type) (b: base_t elt) : GTot nat = U32.v (fst b)
+let base (#elt: Type) (p: ptr elt) : Tot (base_t elt) = (Ghost.reveal p.base_len, p.base)
+let offset (#elt: Type) (p: ptr elt) : Ghost nat (requires True) (ensures (fun offset -> offset <= base_len (base p))) = p.offset
+
+let ptr_base_offset_inj (#elt: Type) (p1 p2: ptr elt) : Lemma
+  (requires (
+    base p1 == base p2 /\
+    offset p1 == offset p2
+  ))
+  (ensures (
+    p1 == p2
+  ))
+= ()
+
+inline_for_extraction // this will extract to ptr, erasing the length field
 [@@noextract_to "krml"]
 noeq
 type array (elt: Type) = {
   p: ptr elt;
-  length: Ghost.erased nat;
-  prf: squash (p.offset + length <= U32.v p.base_len);
+  length: (length: Ghost.erased nat {offset p + length <= base_len (base p)});
 }
 
 let length (#elt: Type) (a: array elt) : GTot nat =
@@ -128,15 +126,18 @@ let change_r_pts_to
   (#carrier: Type u#1)
   (#pcm: P.pcm carrier)
   (p: ref carrier pcm)
-  (v v': carrier)
+  (v: carrier)
+  (p': ref carrier pcm)
+  (v': carrier)
 : SteelGhost unit opened
     (R.pts_to p v)
-    (fun _ -> R.pts_to p v')
-    (fun _ -> v == v')
+    (fun _ -> R.pts_to p' v')
+    (fun _ -> p == p' /\ // keep on 2 distinct lines for error messages
+      v == v')
     (fun _ _ _ -> True)
 = change_equal_slprop
     (R.pts_to p v)
-    (R.pts_to p v')
+    (R.pts_to p' v')
 
 let intro_pts_to (#opened: _) (#elt: Type u#1) (a: array elt) (#v: _) (p: P.perm) (s: Seq.seq elt) : SteelGhost unit opened
   (R.pts_to a.p.base v)
@@ -147,7 +148,7 @@ let intro_pts_to (#opened: _) (#elt: Type u#1) (a: array elt) (#v: _) (p: P.perm
     Seq.length s == length a
   )
   (fun _ _ _ -> True)
-= change_r_pts_to a.p.base v (mk_carrier (U32.v a.p.base_len) a.p.offset s p);
+= change_r_pts_to a.p.base v a.p.base (mk_carrier (U32.v a.p.base_len) a.p.offset s p);
   intro_pure _;
   change_equal_slprop
     (pts_to0 a p s)
@@ -165,27 +166,6 @@ let elim_pts_to (#opened: _) (#elt: Type u#1) (a: array elt) (p: P.perm) (s: Seq
     (pts_to a p s)
     (pts_to0 a p s);
   elim_pure _
-
-(*
-let elim_pts_to_get_base (#opened: _) (#elt: Type u#1) (a: array elt) (p: P.perm) (s: Seq.seq elt) : Steel (ref (carrier_of a) (pcm 
-Ghost.erased (carrier elt (U32.v a.p.base_len))) opened
-  (pts_to a p s)
-  (fun v -> R.pts_to a.p.base v)
-  (fun _ -> True)
-  (fun _ v _ ->
-    Ghost.reveal v == mk_carrier (U32.v a.p.base_len) a.p.offset s p /\
-    valid_perm (U32.v a.p.base_len) a.p.offset (Seq.length s) p /\
-    Seq.length s == length a
-  )
-= let res = Ghost.hide (mk_carrier (U32.v a.p.base_len) a.p.offset s p) in
-  elim_pts_to a p s;
-  change_r_pts_to a.p.base _ res;
-  res
-*)
-
-let change_equal_slprop_by_trefl (#opened:inames) (p q: vprop)
-  : SteelGhost unit opened p (fun _ -> q) (fun _ -> FStar.Tactics.with_tactic FStar.Tactics.trefl (p == q)) (fun h0 _ h1 -> p == q /\ h1 q == h0 p)
-= change_equal_slprop p q
 
 [@@noextract_to "krml"]
 let alloc
@@ -209,12 +189,11 @@ let alloc
   let a = {
     p = p;
     length = Ghost.hide (U32.v n);
-    prf = ();
   }
   in
-  change_equal_slprop_by_trefl
-    (R.pts_to base c)
-    (R.pts_to a.p.base c);
+  change_r_pts_to
+    base c
+    a.p.base c;
   intro_pts_to a P.full_perm (Seq.create (U32.v n) x);
   return a
 
@@ -330,27 +309,6 @@ let gather
   mk_carrier_valid_sum_perm (U32.v a.p.base_len) (a.p.offset) x1 p1 p2;
   intro_pts_to a (p1 `P.sum_perm` p2) x1
 
-let mk_carrier_index
-  (#elt: Type)
-  (len: nat)
-  (offset1: nat)
-  (s1: Seq.seq elt)
-  (p1: P.perm)
-  (i1: nat)
-  (s1': carrier elt)
-  (_: squash (
-    offset1 + Seq.length s1 <= len /\
-    i1 < Seq.length s1 /\
-    P.compatible (pcm elt) (mk_carrier len offset1 s1 p1) s1'
-  ))
-: Lemma
-  (ensures (
-    match M.sel s1' (offset1 + i1) with
-    | None -> False
-    | Some (v, _) -> v == Seq.index s1 i1
-  ))
-= ()
-
 [@@noextract_to "krml"]
 let index
   (#t: Type) (#p: P.perm)
@@ -364,31 +322,9 @@ let index
     (fun _ res _ -> U32.v i < Seq.length s /\ res == Seq.index s (U32.v i))
 = elim_pts_to a p s;
   let s' = R.read a.p.base _ in
-  mk_carrier_index (U32.v a.p.base_len)
-    (a.p.offset) s p (U32.v i) s' ();
   let res = fst (Some?.v (M.sel s' (a.p.offset + U32.v i))) in
   intro_pts_to a p s;
   return res
-
-let mk_carrier_index_simple
-  (#elt: Type)
-  (len: nat)
-  (offset1: nat)
-  (s1: Seq.seq elt)
-  (p1: P.perm)
-  (i1: nat)
-  (_: squash (
-    offset1 + Seq.length s1 <= len /\
-    i1 < Seq.length s1
-  ))
-: Lemma
-  (ensures (
-    let s1' = mk_carrier len offset1 s1 p1 in
-    match M.sel s1' (offset1 + i1) with
-    | None -> False
-    | Some (v, _) -> v == Seq.index s1 i1
-  ))
-= ()
 
 let mk_carrier_upd
   (#elt: Type)
@@ -421,7 +357,6 @@ let upd
     (pts_to a P.full_perm s)
     (fun res -> pts_to a P.full_perm (Seq.upd s (U32.v i) v))
 = elim_pts_to a _ _;
-  mk_carrier_index_simple (U32.v a.p.base_len) a.p.offset s P.full_perm (U32.v i) ();
   mk_carrier_upd (U32.v a.p.base_len) (a.p.offset) s (U32.v i) v ();
   R.upd_gen
     a.p.base
@@ -436,31 +371,22 @@ let upd
     );
   intro_pts_to a _ _
 
-(*
 let adjacent (#elt: Type) (a1 a2: array elt) : Tot prop =
-  a1.p.base_len == a2.p.base_len /\
-  a1.p.base == a2.p.base /\
-  a1.p.offset + a1.length == a2.p.offset
+  base a1.p == base a2.p /\
+  offset a1.p + a1.length == offset a2.p
 
-
-
-inline_for_extraction
+inline_for_extraction // this will extract to "let y = a1"
 [@@noextract_to "krml"]
-let merge (#elt: Type) (a1 a2: array_slice elt)
-: Pure (array_slice elt)
+let merge (#elt: Type) (a1: array elt) (a2: Ghost.erased (array elt))
+: Pure (array elt)
   (requires (adjacent a1 a2))
   (ensures (fun y -> length y == length a1 + length a2))
 = {
-  base = a1.base;
-  base_gr = a1.base_gr;
-  base_inv = a1.base_inv;
-  base_len = a1.base_len;
-  offset = a1.offset;
-  length = U32.add a1.length a2.length;
-  prf = ();
+  p = a1.p;
+  length = a1.length + a2.length;
 }
 
-let merge_assoc (#elt: Type) (a1 a2 a3: array_slice elt) : Lemma
+let merge_assoc (#elt: Type) (a1 a2 a3: array elt) : Lemma
   (requires (adjacent a1 a2 /\ adjacent a2 a3))
   (ensures (
     adjacent (merge a1 a2) a3 /\ adjacent a1 (merge a2 a3) /\
@@ -468,7 +394,7 @@ let merge_assoc (#elt: Type) (a1 a2 a3: array_slice elt) : Lemma
   ))
 = ()
 
-let merge_into (#elt: Type) (a1 a2 a: array_slice elt) : Tot prop =
+let merge_into (#elt: Type) (a1 a2 a: array elt) : Tot prop =
   adjacent a1 a2 /\
   merge a1 a2 == a
 
@@ -494,52 +420,46 @@ let ghost_join
   (#opened: _)
   (#elt: Type)
   (#x1 #x2: Seq.seq elt)
-  (#p: perm)
-  (a1 a2: array_slice elt)
-: STGhost (Ghost.erased (array_slice elt)) opened
+  (#p: P.perm)
+  (a1 a2: array elt)
+: SteelGhost (Ghost.erased (array elt)) opened
     (pts_to a1 p x1 `star` pts_to a2 p x2)
     (fun res -> pts_to res p (x1 `Seq.append` x2))
-    (adjacent a1 a2)
-    (fun res -> merge_into a1 a2 res)
-= rewrite
-    (pts_to a1 p x1)
-    (pts_to0 a1 p x1);
-  rewrite
-    (pts_to a2 p x2)
-    (pts_to0 a2 p x2);
-  let _ = gen_elim () in
-  mk_carrier_merge (A.length a1.base) (U32.v a1.offset) x1 x2 (P.half_perm p);
-  rewrite
-    (R.pts_to a2.base_gr (mk_carrier (A.length a2.base) (U32.v a2.offset) x2 (P.half_perm p)))
-    (R.pts_to a1.base_gr (mk_carrier (A.length a1.base) (U32.v a1.offset + Seq.length x1) x2 (P.half_perm p)));
-  R.gather a1.base_gr
-    (mk_carrier (A.length a1.base) (U32.v a1.offset) x1 (P.half_perm p))
-    (mk_carrier (A.length a1.base) (U32.v a1.offset + Seq.length x1) x2 (P.half_perm p));
+    (fun _ -> adjacent a1 a2)
+    (fun _ res _ -> merge_into a1 a2 res)
+= elim_pts_to a1 p x1;
+  elim_pts_to a2 p x2;
+  mk_carrier_merge (U32.v a1.p.base_len) (a1.p.offset) x1 x2 (p);
+  change_r_pts_to
+    a2.p.base _
+    a1.p.base (mk_carrier (U32.v a1.p.base_len) (a1.p.offset + Seq.length x1) x2 p);
+  R.gather a1.p.base
+    (mk_carrier (U32.v a1.p.base_len) (a1.p.offset) x1 (p))
+    (mk_carrier (U32.v a1.p.base_len) (a1.p.offset + Seq.length x1) x2 (p));
   let res = Ghost.hide (merge a1 a2) in
-  rewrite
-    (R.pts_to a1.base_gr _)
-    (R.pts_to res.base_gr (mk_carrier (A.length res.base) (U32.v res.offset) (x1 `Seq.append` x2) (P.half_perm p)));
-  rewrite
-    (pts_to0 res p (Seq.append x1 x2))
-    (pts_to res p (Seq.append x1 x2));
+  change_r_pts_to
+    a1.p.base _
+    res.p.base (mk_carrier (U32.v res.p.base_len) (res.p.offset) (x1 `Seq.append` x2) (p));
+  intro_pts_to res p (Seq.append x1 x2);
   res
 
-inline_for_extraction
+inline_for_extraction // this will extract to "let res = a1"
 [@@noextract_to "krml"]
 let join
   (#opened: _)
   (#elt: Type)
   (#x1 #x2: Ghost.erased (Seq.seq elt))
-  (#p: perm)
-  (a1 a2: array_slice elt)
-: STAtomicBase (array_slice elt) false opened Unobservable
+  (#p: P.perm)
+  (a1: array elt)
+  (a2: Ghost.erased (array elt))
+: SteelAtomicBase (array elt) false opened Unobservable
     (pts_to a1 p x1 `star` pts_to a2 p x2)
     (fun res -> pts_to res p (x1 `Seq.append` x2))
-    (adjacent a1 a2)
-    (fun res -> merge_into a1 a2 res)
+    (fun _ -> adjacent a1 a2)
+    (fun _ res _ -> merge_into a1 a2 res)
 = let g = ghost_join a1 a2 in
   let res = merge a1 a2 in
-  rewrite
+  change_equal_slprop
     (pts_to g p (x1 `Seq.append` x2))
     (pts_to res p (x1 `Seq.append` x2));
   return res
@@ -564,121 +484,83 @@ let mk_carrier_split
   ))
 = ()
 
+inline_for_extraction // this will extract to "let y = a"
+[@@noextract_to "krml"]
+let split_l (#elt: Type) (a: array elt)
+  (i: Ghost.erased U32.t)
+: Pure (array elt)
+  (requires (U32.v i <= length a))
+  (ensures (fun y -> True))
+= {
+  p = a.p;
+  length = U32.v i;
+}
+
+// TODO: replace with Ghost, introduce pointer shifting operations in SteelAtomicBase Unobservable
+[@@noextract_to "krml"]
+let ptr_shift
+  (#elt: Type)
+  (p: ptr elt)
+  (off: U32.t)
+: Pure (ptr elt)
+  (requires (offset p + U32.v off <= base_len (base p)))
+  (ensures (fun p' ->
+    base p' == base p /\
+    offset p' == offset p + U32.v off
+  ))
+= {
+  base_len = p.base_len;
+  base = p.base;
+  offset = p.offset + U32.v off;
+}
+
 inline_for_extraction
 [@@noextract_to "krml"]
-let tsplit (#elt: Type) (a: array_slice elt)
+let split_r (#elt: Type) (a: array elt)
   (i: U32.t)
-: Pure (array_slice elt & array_slice elt)
+: Pure (array elt)
   (requires (U32.v i <= length a))
-  (ensures (fun y -> merge_into (fst y) (snd y) a))
-= (
-    {
-      base = a.base;
-      base_gr = a.base_gr;
-      base_inv = a.base_inv;
-      base_len = a.base_len;
-      offset = a.offset;
-      length = i;
-      prf = ();
-    }, {
-      base = a.base;
-      base_gr = a.base_gr;
-      base_inv = a.base_inv;
-      base_len = a.base_len;
-      offset = a.offset `U32.add` i;
-      length = a.length `U32.sub` i;
-      prf = ();
-    }
-  )
-    
-#set-options "--ide_id_info_off"
+  (ensures (fun y -> merge_into (split_l a i) y a))
+= {
+  p = ptr_shift a.p i;
+  length = a.length - U32.v i;
+}
 
 let ghost_split
   (#opened: _)
   (#elt: Type)
   (#x: Seq.seq elt)
-  (#p: perm)
-  (a: array_slice elt)
+  (#p: P.perm)
+  (a: array elt)
   (i: U32.t)
-: STGhost (Ghost.erased (array_slice elt & array_slice elt)) opened
+: SteelGhost (squash (U32.v i <= length a /\ U32.v i <= Seq.length x)) opened
     (pts_to a p x)
-    (fun res -> exists_ (fun x1 -> exists_ (fun x2 ->
-      pts_to (fst res) p x1 `star`
-      pts_to (snd res) p x2 `star`
-      pure (
-        U32.v i <= length a /\
-        U32.v i <= Seq.length x /\
-        x1 == Seq.slice x 0 (U32.v i) /\
-        x2 == Seq.slice x (U32.v i) (Seq.length x) /\
-        x == x1 `Seq.append` x2 /\
-        Ghost.reveal res == tsplit a i
-    ))))
-    (U32.v i <= length a)
-    (fun _ -> True)
-= rewrite
-    (pts_to a p x)
-    (pts_to0 a p x);
-  let _ = gen_elim () in
+    (fun res ->
+      pts_to (split_l a i) p (Seq.slice x 0 (U32.v i)) `star`
+      pts_to (split_r a i) p (Seq.slice x (U32.v i) (Seq.length x)))
+    (fun _ -> U32.v i <= length a)
+    (fun _ res _ ->
+      x == Seq.append (Seq.slice x 0 (U32.v i)) (Seq.slice x (U32.v i) (Seq.length x))
+    )
+= 
+  elim_pts_to a p x;
   mk_carrier_split
     (U32.v a.p.base_len)
     (a.p.offset)
     x
-    (P.half_perm p)
+    (p)
     (U32.v i);
   Seq.lemma_split x (U32.v i);
   let xl = Seq.slice x 0 (U32.v i) in
   let xr = Seq.slice x (U32.v i) (Seq.length x) in
-  let vl = mk_carrier (U32.v a.p.base_len) (a.p.offset) xl (P.half_perm p) in
-  let vr = mk_carrier (U32.v a.p.base_len) (a.p.offset + U32.v i) xr (P.half_perm p) in
-  R.share a.base_gr _ vl vr;
-  let res = Ghost.hide (tsplit a i) in
-  rewrite
-    (R.pts_to a.base_gr vl)
-    (R.pts_to (fst res).base_gr (mk_carrier (A.length (fst res).base) (U32.v (fst res).offset) xl (P.half_perm p)));
-  rewrite
-    (pts_to0 (fst res) p xl)
-    (pts_to (fst res) p xl);
-  rewrite
-    (R.pts_to a.base_gr vr)
-    (R.pts_to (snd res).base_gr (mk_carrier (A.length (snd res).base) (U32.v (snd res).offset) xr (P.half_perm p)));
-  rewrite
-    (pts_to0 (snd res) p xr)
-    (pts_to (snd res) p xr);
-  res
-
-inline_for_extraction
-[@@noextract_to "krml"]
-let split
-  (#opened: _)
-  (#elt: Type)
-  (#x: Ghost.erased (Seq.seq elt))
-  (#p: perm)
-  (a: array_slice elt)
-  (i: U32.t)
-: STAtomicBase (array_slice elt & array_slice elt) false opened Unobservable
-    (pts_to a p x)
-    (fun res -> exists_ (fun x1 -> exists_ (fun x2 ->
-      pts_to (fst res) p x1 `star`
-      pts_to (snd res) p x2 `star`
-      pure (
-        U32.v i <= length a /\
-        U32.v i <= Seq.length x /\
-        x1 == Seq.slice x 0 (U32.v i) /\
-        x2 == Seq.slice x (U32.v i) (Seq.length x) /\
-        Ghost.reveal x == x1 `Seq.append` x2 /\
-        res == tsplit a i
-    ))))
-    (U32.v i <= length a)
-    (fun _ -> True)
-= let g = ghost_split a i in
-  let _ = gen_elim () in
-  let res = tsplit a i in
-  let x1 = vpattern_erased (fun x1 -> pts_to (fst g) p x1) in
-  rewrite
-    (pts_to (fst g) p _)
-    (pts_to (fst res) p x1);
-  let x2 = vpattern_erased (fun x2 -> pts_to (snd g) p x2) in
-  rewrite
-    (pts_to (snd g) p _)
-    (pts_to (snd res) p x2);
-  return res
+  let vl = mk_carrier (U32.v a.p.base_len) (a.p.offset) xl (p) in
+  let vr = mk_carrier (U32.v a.p.base_len) (a.p.offset + U32.v i) xr (p) in
+  R.split a.p.base _ vl vr;
+  change_r_pts_to
+    a.p.base vl
+    (split_l a i).p.base vl;
+  intro_pts_to (split_l a i) #vl p (Seq.slice x 0 (U32.v i));
+  change_r_pts_to
+    a.p.base vr
+    (split_r a i).p.base vr;
+  intro_pts_to (split_r a i) #vr p (Seq.slice x (U32.v i) (Seq.length x))
